Low To Mid Done!!

src/specs/PointSubAssign.ec
@@ -60,7 +60,7 @@ module PointSubAssign = {
 
 (* lemma pointSubAssign_extracted_equiv_low :
     equiv [
-      Verifier_1261.usr_pointSubAssign ~ PointSubAssign.low :
+    Verifier_1261.usr_pointSubAssign ~ PointSubAssign.low :
       ={arg, glob PointSubAssign} ==>
       ={res, glob PointSubAssign}
     ].
@@ -71,16 +71,16 @@ proof.
   inline*. wp. skip. by progress.
 qed. *)
 
-op pointSubAssign_memory_footprint (memory: mem) (p1 p2: uint256): mem =
+op pointSubAssign_memory_footprint (memory: mem) (p1 p2 x64 x96: uint256) (result: int*int): mem =
   let point1 = (load memory p1, load memory (p1 + W256.of_int 32)) in
   let point2 = (load memory p2, load memory (p2 + W256.of_int 32)) in
   let mem_1 = store memory W256.zero point1.`1 in
   let mem_2 = store mem_1 (W256.of_int 32) point1.`2 in
-  let mem_3 = store mem_2 (W256.of_int 64) point2.`1 in
-  let mem_4 = store mem_3 (W256.of_int 96) (-(point2.`2) %% (W256.of_int Constants.Q)) in
-  let mem_5 = store mem_4 p1 (ConcretePrimops.ecAdd_precompile_unsafe_cast point1 point2).`1 in
-  store mem_5 (p1 + W256.of_int 32) (ConcretePrimops.ecAdd_precompile_unsafe_cast point1 point2).`2.
-
+  let mem_3 = store mem_2 (W256.of_int 64) x64 in
+  let mem_4 = store mem_3 (W256.of_int 96) x96 in
+  let mem_5 = store mem_4 p1 (W256.of_int result.`1) in
+  store mem_5 (p1 + W256.of_int 32) (W256.of_int result.`2).
+  
 lemma pointSubAssign_low_equiv_mid_fixed (memory: mem) (point_addr_1, point_addr_2: uint256) (point1 point2: int*int) :
     equiv [
       PointSubAssign.low ~ PointSubAssign.mid:
@@ -97,12 +97,13 @@ lemma pointSubAssign_low_equiv_mid_fixed (memory: mem) (point_addr_1, point_addr
       W256.to_uint (load Primops.memory{1} (point_addr_1 + W256.of_int 32)) = point1.`2 /\
       W256.to_uint (load Primops.memory{1} point_addr_2) = point2.`1 /\
       W256.to_uint (load Primops.memory{1} (point_addr_2 + W256.of_int 32)) = point2.`2 /\
+      0 <= point1.`1 < p /\ 0 <= point1.`2 < p /\ 0 <= point2.`1 < p /\ 0 <= point2.`2 < p /\ 
       !Primops.reverted{1}
       ==>
       (Primops.reverted{1} /\ res{2} = None) \/
-      (!Primops.reverted{1} /\ exists p,
+      (!Primops.reverted{1} /\ exists (p: int*int) (x64 x96: uint256),
         res{2} = Some p /\
-        Primops.memory{1} = pointSubAssign_memory_footprint memory point_addr_1 point_addr_2
+        Primops.memory{1} = pointSubAssign_memory_footprint memory point_addr_1 point_addr_2 x64 x96 p
       )
     ].
     proof.
@@ -112,15 +113,42 @@ lemma pointSubAssign_low_equiv_mid_fixed (memory: mem) (point_addr_1, point_addr
       pose point2_x := load memory point_addr_2.
       pose point2_y := load memory (point_addr_2 + W256.of_int 32).
       pose mem_1 := store memory W256.zero point1_x.
+      have H_mem_1_point_x : forall (point: uint256), 128 <= W256.to_uint point /\ 64 <= W256.to_uint(-point) => load mem_1 point = load memory point.
+      progress. rewrite load_store_diff. smt(@W256 @Utils). smt (@W256 @Utils). reflexivity.
+      have H_mem_1_point_y : forall (point: uint256), 128 <= W256.to_uint point /\ 64 <= W256.to_uint(-point) => load mem_1 (point + W256.of_int 32) = load memory (point + W256.of_int 32).
+      progress. rewrite load_store_diff. smt(@W256 @Utils). smt (@W256 @Utils). reflexivity.
       pose mem_2 := store mem_1 (W256.of_int 32) point1_y.
+      have H_mem_2_point_x : forall (point: uint256), 128 <= W256.to_uint point /\ 64 <= W256.to_uint(-point) => load mem_2 point = load memory point.
+      progress. rewrite load_store_diff. smt(@W256 @Utils). smt (@W256 @Utils). exact H_mem_1_point_x.
+      have H_mem_2_point_y : forall (point: uint256), 128 <= W256.to_uint point /\ 64 <= W256.to_uint(-point) => load mem_2 (point + W256.of_int 32) = load memory (point + W256.of_int 32).
+      progress. rewrite load_store_diff. smt(@W256 @Utils). smt (@W256 @Utils). exact H_mem_1_point_y.
       pose mem_3 := store mem_2 (W256.of_int 64) point2_x.
+      have H_mem_3_point_x : forall (point: uint256), 128 <= W256.to_uint point /\ 64 <= W256.to_uint(-point) => load mem_3 point = load memory point.
+      progress. rewrite load_store_diff. smt(@W256 @Utils). smt (@W256 @Utils). exact H_mem_2_point_x.
+      have H_mem_3_point_y : forall (point: uint256), 128 <= W256.to_uint point /\ 64 <= W256.to_uint(-point) => load mem_3 (point + W256.of_int 32) = load memory (point + W256.of_int 32).
+      progress. rewrite load_store_diff. smt(@W256 @Utils). smt (@W256 @Utils). exact H_mem_2_point_y.
       pose mem_4 := store mem_3 (W256.of_int 96) point2_y.
-      seq 2 0: (
+      have H_mem_4_point_x : forall (point: uint256), 128 <= W256.to_uint point /\ 64 <= W256.to_uint(-point) => load mem_4 point = load memory point.
+      progress. rewrite load_store_diff. smt(@W256 @Utils). smt (@W256 @Utils). exact H_mem_3_point_x.
+      have H_mem_4_point_y : forall (point: uint256), 128 <= W256.to_uint point /\ 64 <= W256.to_uint(-point) => load mem_4 (point + W256.of_int 32) = load memory (point + W256.of_int 32).
+      progress. rewrite load_store_diff. smt(@W256 @Utils). smt (@W256 @Utils). exact H_mem_3_point_y.
+      have H_mem_4_0: load mem_4 W256.zero = point1_x.
+      rewrite load_store_diff. smt (@W256 @Utils). smt (@W256 @Utils).
+      rewrite load_store_diff. smt (@W256 @Utils). smt (@W256 @Utils).
+      rewrite load_store_diff. smt (@W256 @Utils). smt (@W256 @Utils).
+      rewrite load_store_same. reflexivity.
+      have H_mem_4_32: load mem_4 (W256.of_int 32) = point1_y.
+      rewrite load_store_diff. smt (@W256 @Utils). smt (@W256 @Utils).
+      rewrite load_store_diff. smt (@W256 @Utils). smt (@W256 @Utils).
+      rewrite load_store_same. reflexivity.
+      have H_mem_4_64: load mem_4 (W256.of_int 64) = point2_x. rewrite load_store_diff. smt (@W256 @Utils). smt (@W256 @Utils). rewrite load_store_same. reflexivity.
+      have H_mem_4_96: load mem_4 (W256.of_int 96) = point2_y. rewrite load_store_same. reflexivity.
+      seq 8 0: (
         p1{1} = point_addr_1 /\
         p2{1} = point_addr_2 /\
         p1{2} = point1 /\
         p2{2} = point2 /\
-        Primops.memory{1} = mem_1 /\
+        Primops.memory{1} = mem_4 /\
         128 <= W256.to_uint point_addr_1 /\
         128 <= W256.to_uint point_addr_2 /\
         64 <= W256.to_uint (-point_addr_1) /\
@@ -129,295 +157,143 @@ lemma pointSubAssign_low_equiv_mid_fixed (memory: mem) (point_addr_1, point_addr
         W256.to_uint (load Primops.memory{1} (point_addr_1 + W256.of_int 32)) = point1.`2 /\
         W256.to_uint (load Primops.memory{1} point_addr_2) = point2.`1 /\
         W256.to_uint (load Primops.memory{1} (point_addr_2 + W256.of_int 32)) = point2.`2 /\
+        p1{2}.`1 = W256.to_uint point1_x /\
+        p1{2}.`2 = W256.to_uint point1_y /\
+        p2{2}.`1 = W256.to_uint point2_x /\
+        p2{2}.`2 = W256.to_uint point2_y /\
+        0 <= point1.`1 < p /\ 0 <= point1.`2 < p /\ 0 <= point2.`1 < p /\ 0 <= point2.`2 < p /\ 
        !Primops.reverted{1}
-      ).
-      call{1} (ConcretePrimops.mstore_pspec memory W256.zero point1_x).
-      call{1} (ConcretePrimops.mload_pspec memory point_addr_1).
-      skip. progress.
-      rewrite load_store_diff. smt(@W256 @Utils). smt(@W256 @Utils). smt ().
-      rewrite load_store_diff. smt(@W256 @Utils). smt(@W256 @Utils). smt ().
-      rewrite load_store_diff. smt(@W256 @Utils). smt(@W256 @Utils). smt ().
-      rewrite load_store_diff. smt(@W256 @Utils). smt(@W256 @Utils). smt ().
-      seq 2 0: (
-        p1{1} = point_addr_1 /\
-        p2{1} = point_addr_2 /\
-        p1{2} = point1 /\
-        p2{2} = point2 /\
-        Primops.memory{1} = mem_2 /\
-        128 <= W256.to_uint point_addr_1 /\
-        128 <= W256.to_uint point_addr_2 /\
-        64 <= W256.to_uint (-point_addr_1) /\
-        64 <= W256.to_uint (-point_addr_2) /\
-        W256.to_uint (load Primops.memory{1} point_addr_1) = point1.`1 /\
-        W256.to_uint (load Primops.memory{1} (point_addr_1 + W256.of_int 32)) = point1.`2 /\
-        W256.to_uint (load Primops.memory{1} point_addr_2) = point2.`1 /\
-        W256.to_uint (load Primops.memory{1} (point_addr_2 + W256.of_int 32)) = point2.`2 /\
-       !Primops.reverted{1}
-      ).
-      call{1} (ConcretePrimops.mstore_pspec mem_1 (W256.of_int 32) point1_y).
-      call{1} (ConcretePrimops.mload_pspec mem_1 (point_addr_1 + W256.of_int 32)).
-      skip. progress.
-      rewrite load_store_diff. smt(@W256 @Utils). smt(@W256 @Utils). smt ().
-      rewrite load_store_diff. smt(@W256 @Utils). smt(@W256 @Utils). smt ().
-      rewrite load_store_diff. smt(@W256 @Utils). smt(@W256 @Utils). smt ().
-      rewrite load_store_diff. smt(@W256 @Utils). smt(@W256 @Utils). smt ().
-      rewrite load_store_diff. smt(@W256 @Utils). smt(@W256 @Utils). smt ().
-      seq 2 0: (
-        p1{1} = point_addr_1 /\
-        p2{1} = point_addr_2 /\
-        p1{2} = point1 /\
-        p2{2} = point2 /\
-        Primops.memory{1} = mem_3 /\
-        128 <= W256.to_uint point_addr_1 /\
-        128 <= W256.to_uint point_addr_2 /\
-        64 <= W256.to_uint (-point_addr_1) /\
-        64 <= W256.to_uint (-point_addr_2) /\
-        W256.to_uint (load Primops.memory{1} point_addr_1) = point1.`1 /\
-        W256.to_uint (load Primops.memory{1} (point_addr_1 + W256.of_int 32)) = point1.`2 /\
-        W256.to_uint (load Primops.memory{1} point_addr_2) = point2.`1 /\
-        W256.to_uint (load Primops.memory{1} (point_addr_2 + W256.of_int 32)) = point2.`2 /\
-       !Primops.reverted{1}
-      ).
+    ).
+      call{1} (ConcretePrimops.mstore_pspec mem_3 (W256.of_int 96) point2_y).
+      call{1} (ConcretePrimops.mload_pspec mem_3 (point_addr_2 + W256.of_int 32)).
       call{1} (ConcretePrimops.mstore_pspec mem_2 (W256.of_int 64) point2_x).
       call{1} (ConcretePrimops.mload_pspec mem_2 point_addr_2).
-      skip. progress.
-      rewrite load_store_diff. smt(@W256 @Utils). smt(@W256 @Utils). smt ().
-      rewrite load_store_diff. smt(@W256 @Utils). smt(@W256 @Utils). smt ().
-      rewrite load_store_diff. smt(@W256 @Utils). smt(@W256 @Utils). smt ().
-      rewrite load_store_diff. smt(@W256 @Utils). smt(@W256 @Utils). smt ().
-      rewrite load_store_diff. smt(@W256 @Utils). smt(@W256 @Utils). smt ().      
-
-
-
-
-
-
-
-
-
-
-
-
-
-
-
-
-
-          call{1} (ConcretePrimops.mstore_pspec mem_3 (W256.of_int 96) point2_y).
-        call{1} (ConcretePrimops.mload_pspec mem_3 (point_addr_2 + W256.of_int 32)).
-
-
-
+      call{1} (ConcretePrimops.mstore_pspec mem_1 (W256.of_int 32) point1_y).
+      call{1} (ConcretePrimops.mload_pspec mem_1 (point_addr_1 + W256.of_int 32)).
+      call{1} (ConcretePrimops.mstore_pspec memory W256.zero point1_x).
+      call{1} (ConcretePrimops.mload_pspec memory point_addr_1).
         skip. progress.
-        rewrite load_store_diff. smt(@W256 @Utils). smt(@W256 @Utils). smt().
-        rewrite load_store_diff. smt(@W256 @Utils). smt(@W256 @Utils).
-        rewrite load_store_diff. smt(@W256 @Utils). smt(@W256 @Utils). smt ().
-        rewrite load_store_diff. smt(@W256 @Utils). smt(@W256 @Utils).
-        rewrite load_store_diff. smt(@W256 @Utils). smt(@W256 @Utils).
-        rewrite load_store_diff. smt(@W256 @Utils). smt(@W256 @Utils). smt ().
-        rewrite load_store_diff.
-        clear H20 H19 H18 H17 H16 H15 H14 H13 H12 H11 H10 H9 H8 H7. smt (@W256 @Utils).
-        clear H20 H19 H18 H17 H16 H15 H14 H13 H12 H11 H10 H9 H8 H7. smt (@W256 @Utils).
-        rewrite load_store_diff. smt(@W256 @Utils). smt(@W256 @Utils).
-        rewrite load_store_diff. clear H20 H18 H16 H14. smt(@W256 @Utils). smt(@W256 @Utils).
-        rewrite load_store_diff. smt(@W256 @Utils). smt(@W256 @Utils).
-      case (point2_y = W256.zero /\ point2_x <> W256.zero).
-          seq 0 2: (ret{2} = None).
-          inline PointNegate.mid.
-          rcondt{2} 2. progress. wp. skip. progress.
-
-
-
-
-lemma pointSubAssign_low_equiv_mid_fail_case (memory: mem) (point_addr_1, point_addr_2: uint256) (point1 point2: int*int) :
-    point2.`2 = 0 =>
-    equiv [
-      PointSubAssign.low ~ PointSubAssign.mid:
-      arg{1}.`1 = point_addr_1 /\
-      arg{1}.`2 = point_addr_2 /\
-      arg{2}.`1 = point1 /\
-      arg{2}.`2 = point2 /\
-      Primops.memory{1} = memory /\
-      128 <= W256.to_uint point_addr_1 /\
-      128 <= W256.to_uint point_addr_2 /\
-      64 <= W256.to_uint (-point_addr_1) /\
-      64 <= W256.to_uint (-point_addr_2) /\
-      W256.to_uint (load Primops.memory{1} point_addr_1) = point1.`1 /\
-      W256.to_uint (load Primops.memory{1} (point_addr_1 + W256.of_int 32)) = point1.`2 /\
-      W256.to_uint (load Primops.memory{1} point_addr_2) = point2.`1 /\
-      W256.to_uint (load Primops.memory{1} (point_addr_2 + W256.of_int 32)) = point2.`2 /\
-      !Primops.reverted{1}
-      ==>
-      (Primops.reverted{1} /\ res{2} = None) \/
-      (!Primops.reverted{1} /\ exists p,
-        res{2} = Some p /\
-        Primops.memory{1} = pointSubAssign_memory_footprint memory
+        exact H_mem_1_point_y. exact H_mem_2_point_x. exact H_mem_3_point_y.
+        rewrite - / mem_4. rewrite H_mem_4_point_x. smt (). smt ().
+        rewrite - /mem_4. rewrite H_mem_4_point_y. smt (). smt ().
+        rewrite - / mem_4. rewrite H_mem_4_point_x. smt (). smt ().
+        rewrite - /mem_4. rewrite H_mem_4_point_y. smt (). smt ().
+        smt (). smt (). smt (). smt ().
+    seq 1 1: (
+      (Primops.reverted{1} /\ neg_p2_opt{2} = None) \/
+      (
+        p1{1} = point_addr_1 /\
+        !Primops.reverted{1} /\
+        p1{2}.`1 = W256.to_uint point1_x /\
+        p1{2}.`2 = W256.to_uint point1_y /\
+        p2{2}.`1 = W256.to_uint point2_x /\
+        p2{2}.`2 = W256.to_uint point2_y /\
+        0 <= p1{2}.`1 < p /\ 0 <= p1{2}.`2 < p /\ 0 <= p2{2}.`1 < p /\ 0 <= p2{2}.`2 < p /\
+        exists neg_point,
+          neg_p2_opt{2} = Some neg_point /\
+          0 <= neg_point.`1 < Constants.Q /\ 0 <= neg_point.`2 < Constants.Q /\
+          Primops.memory{1} = store (store mem_4 (W256.of_int 64) (W256.of_int neg_point.`1)) (W256.of_int 96) (W256.of_int neg_point.`2)
       )
-    ].
-    proof.
-    move=>H_y_eq_0.
-      proc.
-      seq 9 0: (load Primops.memory{1} (W256.of_int 96) = W256.of_int Constants.Q /\ p2{2} = point2).
-      inline Primops.gas. wp.
-      inline Primops.mstore Primops.mload. wp. skip.
-      progress.
-      pose mem_1 := store Primops.memory{1} W256.zero (load Primops.memory{1} p1{1}).
-      pose mem_2 := store mem_1 (W256.of_int 32) (load mem_1 (p1{1} + W256.of_int 32)).
-      pose mem_3 := store mem_2 (W256.of_int 64) (load mem_2 p2{1}).
-      rewrite load_store_same.
-      have H_load_eq_0 : load mem_3 (p2{1} + (W256.of_int 32)) = W256.zero.
-      rewrite /mem_3. rewrite load_store_diff. smt (@W256 @Utils). smt (@W256 @Utils).
-      rewrite /mem_2. rewrite load_store_diff. smt (@W256 @Utils). smt (@W256 @Utils).
-      rewrite /mem_1. rewrite load_store_diff. smt (@W256 @Utils). smt (@W256 @Utils).
-      smt (@W256 @Utils).
-      rewrite H_load_eq_0. smt (@W256 @Utils).
-      seq 1 0: (_16{1} = W256.zero /\ p2{2} = point2).
-      exists* Primops.memory{1}.
-      elim*=>memory_pre_staticcall.
-      exists* p1{1}.
-      elim*=>p1_addr.
-      call{1} (
-        ConcretePrimops.staticcall_ec_add_pspec
-        memory_pre_staticcall
-        ((load memory_pre_staticcall W256.zero),
-        (load memory_pre_staticcall (W256.of_int 32)))
-        ((load memory_pre_staticcall (W256.of_int 64)),
-        W256.of_int Constants.Q)
-        W256.zero
-        p1_addr
-      ).
-          skip.
-          progress. smt ().
-          have H_staticcall_should_not_success : forall (a b c: uint256), ! (ConcretePrimops.staticcall_ec_add_should_succeed (a, b) (c, W256.of_int Constants.Q)).
-          progress. rewrite /ConcretePrimops.staticcall_ec_add_should_succeed.
-          have H_not_wellformed: !ConcretePrimops.point_wellformed(c, W256.of_int Constants.Q).
-          rewrite /point_wellformed.
-          simplify.
-          have H_Q_neq_q_mod_p : W256.of_int Constants.Q <> (W256.of_int Constants.Q %% W256.of_int p).
-          rewrite Constants.q_eq_elliptic_curve_p. rewrite /W256.\umod. rewrite /W256.ulift2. smt. smt(). smt(). smt().
-      rcondt{1} 1. progress. skip. rewrite /iszero /bool_of_uint256. progress. smt (@W256 @Utils).
-      call{1} revertWithMessage_low_pspec.
-      rcondt{2} 1. by progress.
-      wp. skip. by progress.
-    qed.
-
-  lemma pointSubAssign_low_equiv_mid_success_case (memory: mem) (point_addr_1, point_addr_2) (point1 point2: int*int) :
-      point2.`2 <> 0 =>
-      equiv [
-        PointSubAssign.low ~ PointSubAssign.mid:
-        arg{1}.`1 = point_addr_1 /\
-        arg{1}.`2 = point_addr_2 /\
-        arg{2}.`1 = point1 /\
-        arg{2}.`2 = point2 /\
-        0 <= point1.`1 < p /\ 0 <= point1.`2 < p /\ 0 <= point2.`1 < p /\ 0 <= point2.`2 < p /\
-        Primops.memory{1} = memory /\
-        128 <= W256.to_uint point_addr_1 /\
-        128 <= W256.to_uint point_addr_2 /\
-        64 <= W256.to_uint (-point_addr_1) /\
-        64 <= W256.to_uint (-point_addr_2) /\
-        W256.to_uint (load Primops.memory{1} point_addr_1) = point1.`1 /\
-        W256.to_uint (load Primops.memory{1} (point_addr_1 + W256.of_int 32)) = point1.`2 /\
-        W256.to_uint (load Primops.memory{1} point_addr_2) = point2.`1 /\
-        W256.to_uint (load Primops.memory{1} (point_addr_2 + W256.of_int 32)) = point2.`2 /\
-        !Primops.reverted{1}
-        ==>
-        (Primops.reverted{1} /\ res{2} = None) \/
-        (!Primops.reverted{1} /\ exists p,
-          res{2} = Some p /\
-          Primops.memory{1} = pointSubAssign_memory_footprint memory
-        )
-      ].
-      proof.
-      move=> H_y_neq_0.
-        proc.
-        rcondf{2} 1. by progress.
-        inline PointNegate.mid.
-        sp. simplify.
-        inline PointAddIntoDest.mid.
-        pose mem_1 := store memory W256.zero (load memory point_addr_1).
-        pose mem_2 := store mem_1 (W256.of_int 32) (load memory (point_addr_1 + W256.of_int 32)).
-        pose mem_3 := store mem_2 (W256.of_int 64) (load memory point_addr_2).
-        pose mem_4 := store mem_3 (W256.of_int 96) (W256.of_int Constants.Q - (load memory (point_addr_2 + W256.of_int 32))).
-        seq 9 0: (
-          Primops.memory{1} = mem_4 /\
-          p1{1} = point_addr_1 /\
-          W256.to_uint (load memory point_addr_1) = point1.`1 /\
-          W256.to_uint (load memory (point_addr_1 + W256.of_int 32)) = point1.`2 /\
-          W256.to_uint (load memory point_addr_2) = point2.`1 /\
-          W256.to_uint (load memory (point_addr_2 + W256.of_int 32)) = point2.`2 /\
-          0 <= point1.`1 < p /\ 0 <= point1.`2 < p /\ 0 <= point2.`1 < p /\ 0 <= point2.`2 < p
-        ).
-        inline Primops.gas. wp.
-        call{1} (ConcretePrimops.mstore_pspec mem_3 (W256.of_int 96) (W256.of_int Constants.Q - (load memory (point_addr_2 + W256.of_int 32)))).
-        call{1} (ConcretePrimops.mload_pspec mem_3 (point_addr_2 + W256.of_int 32)).
-        call{1} (ConcretePrimops.mstore_pspec mem_2 (W256.of_int 64) (load memory point_addr_2)).
-        call{1} (ConcretePrimops.mload_pspec mem_2 point_addr_2).
-        call{1} (ConcretePrimops.mstore_pspec mem_1 (W256.of_int 32) (load memory (point_addr_1 + W256.of_int 32))).
-        call{1} (ConcretePrimops.mload_pspec mem_1 (point_addr_1 + W256.of_int 32)).
-        call{1} (ConcretePrimops.mstore_pspec memory W256.zero (load memory point_addr_1)).
-        call{1} (ConcretePrimops.mload_pspec memory point_addr_1).
-        skip.
-        progress. smt (). smt().
-        rewrite load_store_diff. smt (@W256 @Utils). smt (@W256 @Utils). reflexivity.
-        smt ().
-        rewrite load_store_diff. smt (@W256 @Utils). smt (@W256 @Utils).
-        rewrite load_store_diff. smt (@W256 @Utils). smt (@W256 @Utils). reflexivity.
-        rewrite load_store_diff. smt (@W256 @Utils). smt (@W256 @Utils).
-        rewrite load_store_diff. smt (@W256 @Utils). smt (@W256 @Utils).
-        rewrite load_store_diff. smt (@W256 @Utils). smt (@W256 @Utils). reflexivity.
-        smt (). smt(). smt(). smt(). smt (). smt (). smt (). smt (). smt (). smt (). smt (). smt ().
-        seq 1 0: (_16{1} = W256.one).
-        exists* Primops.memory{1}, p1{1}.
-        elim* => memory_pre_staticcall p_addr_1.
-        call{1} (
-          ConcretePrimops.staticcall_ec_add_pspec
-          memory_pre_staticcall
-          (load memory_pre_staticcall W256.zero, load memory_pre_staticcall (W256.of_int 32))
-          (load memory_pre_staticcall (W256.of_int 64), load memory_pre_staticcall (W256.of_int 96))
-          W256.zero
-          p_addr_1
-        ).
-            skip.
-            progress.
-            have H_should_succeed: ConcretePrimops.staticcall_ec_add_should_succeed
-              ((load mem_4 W256.zero), (load mem_4 (W256.of_int 32)))
-              ((load mem_4 (W256.of_int 64)), (load mem_4 (W256.of_int 96))).
-                rewrite load_store_diff. smt (@W256 @Utils). smt (@W256 @Utils).
-                rewrite load_store_diff. smt (@W256 @Utils). smt (@W256 @Utils).
-                rewrite load_store_diff. smt (@W256 @Utils). smt (@W256 @Utils).
-                rewrite load_store_same.
-                rewrite load_store_diff. smt (@W256 @Utils). smt (@W256 @Utils).
-                rewrite load_store_diff. smt (@W256 @Utils). smt (@W256 @Utils).
-                rewrite load_store_same.
-                rewrite load_store_diff. smt (@W256 @Utils). smt (@W256 @Utils).
-                rewrite load_store_same.
-                rewrite load_store_same.
-                rewrite /staticcall_ec_add_should_succeed.
-                rewrite /point_wellformed. progress. rewrite - W256.to_uintK H. rewrite /W256.\umod /W256.ulift2. rewrite W256.of_uintK W256.of_uintK.
-                rewrite pmod_small. progress. smt (@W256 @Utils @IntDiv).
-                rewrite pmod_small. progress. smt (@Constants).
-                rewrite pmod_small. progress. smt (@Constants). smt(@Constants). smt().
-                rewrite pmod_small. smt (@Constants @W256 @Utils @IntDiv). reflexivity.
-                rewrite - W256.to_uintK. rewrite H0. smt (@Constants @W256 @IntDiv @Utils).
-                rewrite - W256.to_uintK H1. smt (@Constants @W256 @IntDiv @Utils).
-                rewrite /W256.\umod /W256.ulift2. rewrite W256.of_uintK.
-                rewrite pmod_small. progress. smt (@W256).
-                rewrite pmod_small. smt (@Constants).
-                have H_y: load memory (point_addr_2 + (W256.of_int 32)) = W256.of_int point2.`2. smt (@W256 @Utils).
-                rewrite H_y. smt (@Constants @W256 @Utils).
-                smt (@W256).
-                
-
-
-
-              
-                rewrite - W256.to_uintK. smt (@Constants @W256 @IntDiv @Utils).
-                simplify.
-                rewrite /point_wellformed.
-                simplify.
-                do rewrite H.
-                do rewrite H1.
-                do rewrite H2.
-        
-      
+    ).
+    call{1} (pointNegate_low_equiv_mid mem_4 (W256.of_int 64) point2.`1 point2.`2).
+    skip. progress. smt (). smt (@Constants). smt (@Constants). smt (). smt (). smt ().
     
+    case (Primops.reverted{1}).
+      rcondt{2} 1. progress. skip. progress. smt ().
+      inline Primops.gas. sp.
+      seq 1 0: (Primops.reverted{1} /\ ret{2} = None). call{1} (ConcretePrimops.staticcall_pspec_revert). skip. by progress.
+      if{1}. call{1} (revertWithMessage_low_pspec). skip. by progress.
+      skip. by progress.
+    (* !Primops.reverted{1} *)
+      rcondf{2} 1. progress. skip. progress. smt ().
+      inline PointAddIntoDest.mid.
+      inline Primops.gas Primops.staticcall.
+      rcondf{1} 8. progress. wp. skip. progress. smt (@W256 @Utils).
+      rcondt{1} 8. progress. wp. skip. by progress.
+      rcondt{1} 8. progress. wp. skip. by progress.
+      seq 11 5: (
+        x1{2} = W256.to_uint x1{1} /\
+        x2{2} = W256.to_uint x2{1} /\
+        y1{2} = W256.to_uint y1{1} /\
+        y2{2} = W256.to_uint y2{1} /\
+        0 <= x1{2} < p /\ 0 <= x2{2} < p /\ 0 <= y1{2} < p /\ 0 <= y2{2} < p /\
+        Primops.memory{1} = store (store mem_4 (W256.of_int 64) x2{1}) (W256.of_int 96) y2{1} /\
+        !Primops.reverted{1} /\
+        retOff{1} = point_addr_1
+      ).
+        inline Primops.mload. wp. skip.
+        move=> &1 &2 H.
+        have H_post_negate: exists neg_point,
+          neg_p2_opt{2} = Some neg_point /\
+          0 <= neg_point.`1 < Constants.Q /\ 0 <= neg_point.`2 < Constants.Q /\
+          Primops.memory{1} = store (store mem_4 (W256.of_int 64) (W256.of_int neg_point.`1)) (W256.of_int 96) (W256.of_int neg_point.`2).
+            smt ().
+        case H_post_negate.
+        move => neg_point H_post_negate.
+        pose mem_post_negate := store (store mem_4 (W256.of_int 64) (W256.of_int neg_point.`1)) (W256.of_int 96) (W256.of_int neg_point.`2).
+        have H_mem_post_negate: Primops.memory{1} = mem_post_negate. smt ().
+        rewrite H_mem_post_negate.
+        progress.
+        rewrite load_store_diff. smt (@W256 @Utils). smt (@W256 @Utils).
+        rewrite load_store_diff. smt (@W256 @Utils). smt (@W256 @Utils).
+        rewrite H_mem_4_0. smt ().
+        rewrite load_store_diff. smt (@W256 @Utils). smt (@W256 @Utils).
+        rewrite load_store_same. rewrite W256.of_uintK. rewrite pmod_small. smt (). smt ().
+        rewrite load_store_diff. smt (@W256 @Utils). smt (@W256 @Utils).
+        rewrite load_store_diff. smt (@W256 @Utils). smt (@W256 @Utils).
+        rewrite H_mem_4_32. smt ().
+        rewrite load_store_same. smt (@W256 @Utils @Constants).
+          smt (). smt (). smt (). smt (@Constants). smt (). smt (@Constants). smt (). smt (@Constants).
+        rewrite /mem_post_negate. rewrite load_store_same. congr. congr. rewrite load_store_diff. smt (@W256 @Utils). smt (@W256 @Utils). rewrite load_store_same. reflexivity. smt (). smt ().
+      rcondf{1} 5. progress. wp. skip. progress.
+      have H_x1: x1{hr} = x1{hr} %% (W256.of_int p).
+        rewrite /W256.\umod /W256.ulift2. rewrite W256.of_uintK. rewrite pmod_small. progress. rewrite pmod_small. progress.
+        smt (@Constants). smt (@Constants). smt (). rewrite W256.to_uintK. reflexivity.
+      have H_y1: y1{hr} = y1{hr} %% (W256.of_int p).
+        rewrite /W256.\umod /W256.ulift2. rewrite W256.of_uintK. rewrite pmod_small. progress. rewrite pmod_small. progress.
+        smt (@Constants). smt (@Constants). smt (). rewrite W256.to_uintK. reflexivity.
+      have H_x2: x2{hr} = x2{hr} %% (W256.of_int p).
+        rewrite /W256.\umod /W256.ulift2. rewrite W256.of_uintK. rewrite pmod_small. progress. rewrite pmod_small. progress.
+        smt (@Constants). smt (@Constants). smt (). rewrite W256.to_uintK. reflexivity.
+      have H_y2: y2{hr} = y2{hr} %% (W256.of_int p).
+        rewrite /W256.\umod /W256.ulift2. rewrite W256.of_uintK. rewrite pmod_small. progress. rewrite pmod_small. progress.
+        smt (@Constants). smt (@Constants). smt (). rewrite W256.to_uintK. reflexivity.
+        smt ().
+      
+      seq 4 4: (
+        #pre /\
+        ={x1_F, y1_F, x2_F, y2_F} /\
+        x1_F{2} = ZModField.inzmod x1{2} /\
+        y1_F{2} = ZModField.inzmod y1{2} /\
+        x2_F{2} = ZModField.inzmod x2{2} /\
+        y2_F{2} = ZModField.inzmod y2{2}
+      ). wp. skip. by progress.
+      if{1}.
+      (*failure case*)
+        rcondt{1} 3. progress. wp. skip. progress. rewrite /iszero /bool_of_uint256. smt (@W256 @Utils).
+        call{1} (revertWithMessage_low_pspec). wp. skip. progress. left. progress. smt (@EllipticCurve).
+      (*success case*)
+        seq 1 1: (#pre /\ ={result} (* /\ result{1} = ecAdd_precompile x1_F{1} y1_F{1} x2_F{1} y2_F{1}*) ). wp. skip. by progress.
+        if{1}. sp. rcondt{1} 1. progress. skip. progress. rewrite /iszero /bool_of_uint256. smt (@W256 @Utils).
+          call{1} (revertWithMessage_low_pspec). wp. skip. progress. left. progress.
+          have H_none: forall (a: (F*F) option), is_none a => a = None. smt ().
+          smt ().
+        inline Primops.mstore. sp.
+        rcondf{1} 1. progress. skip. progress. rewrite /iszero /bool_of_uint256. smt ().
+        skip. progress.
+        right.
+        progress.
+          rewrite /pointSubAssign_memory_footprint. progress.
+          rewrite /mem_4 /mem_3.
+          rewrite (store_store_swap_diff mem_2 _ _ _ _). smt (@W256 @Utils). smt (@W256 @Utils).
+          rewrite store_store_same. rewrite (store_store_swap_diff mem_2 _ _ _ _). smt (@W256 @Utils). smt (@W256 @Utils).
+          rewrite /mem_2 /mem_1. rewrite - /point1_x. rewrite - /point1_y.
+          rewrite store_store_same.
+          exists (topoint (odflt (ZModField.zero, ZModField.zero) result{2})).
+          exists x2{1}.
+          exists y2{1}.
+          progress.
+          have H_res: exists (r: F*F), result{2} = Some r. smt ().
+          case H_res. by progress.
+      qed.
+
